\begin{enumerate}[label=\thesubsection.\arabic*,ref=\thesubsection.\theenumi]
	\item Find the sum
\begin{align}
	\label{eq:ap-sum10}
	S = 1 + 2 + \dots + 10
\end{align}
\solution Reversing the sum in
	\eqref{eq:ap-sum10}
	as
\begin{align}
	\label{eq:ap-sum10-rev}
	S = 10 + 9 + \dots + 1
\end{align}
and adding 
	\eqref{eq:ap-sum10}
	and
	\eqref{eq:ap-sum10-rev},
\begin{align}
	\label{eq:ap-sum10-add}
	2S &= 11 + 11 + \dots + 11 \quad 10 \text{ times}
	\\
	\implies S &= \frac{11 \times 10}{2} = 55
\end{align}
\item The sum of the first $n$ natural numbers is
\begin{align}
	\sum_{k=1}^{n}k &= 1+ 2 + \dots + n
	\\
	&= \frac{n\brak{n+1}}{2}
	\label{eq:ap-sumn}
\end{align}
\item The $n^{th}$ term of an arithmetic progression (AP) is
\begin{align}
	\label{eq:ap-nthterm}
	x(n) = x(0) + nd, \quad n = 0, 1, \dots
\end{align}
\item 
\begin{align}
	\label{eq:ap-nsum}
	 y(n)=\sum_{k=0}^{n}x(k) = \frac{n+1}{2}\brak{x(0) + \frac{dn}{2}}
\end{align}
\solution
From
	\eqref{eq:ap-nthterm}
	and
	\eqref{eq:ap-nsum},
\begin{align}
	\label{eq:ap-nthsum}
	 \sum_{k=0}^{n}x(k) &= 
\sum_{k=0}^{n}
	 \brak{x(0) + kd} 
	 \\
	 &= 
\sum_{k=0}^{n}x(0) + 
d\sum_{k=1}^{n}k
	  = \brak{n+1}x(0) + d\frac{n\brak{n+1}}{2}
\end{align}
upon substituting from
	\eqref{eq:ap-sumn}, yielding
	\eqref{eq:ap-nthsum}
	upon simplification.
\end{enumerate}
